new folder for setoid rewriting that abstracts the extensional equality

case-studies/kathrin/coq-setoid-funcomp/Chapter3/utlc_pure.v
@@ -1,4 +1,10 @@
-Require Import core core_axioms unscoped unscoped_axioms.
+Require Import core unscoped.
+
+Require Import core_axioms unscoped_axioms.
+Require Import Setoid Morphisms Relation_Definitions.
+
+Module renSubst.
+
 Inductive tm : Type :=
   | var_tm : nat -> tm
   | app : tm -> tm -> tm
@@ -75,7 +81,7 @@ Fixpoint extRen_tm (xi_tm : nat -> nat) (zeta_tm : nat -> nat)
 (Eq_tm : forall x, xi_tm x = zeta_tm x) (s : tm) {struct s} :
 ren_tm xi_tm s = ren_tm zeta_tm s :=
   match s with
-  | var_tm s0 => ap var_tm (Eq_tm s0)
+  | var_tm s0 => ap (var_tm) (Eq_tm s0)
   | app s0 s1 =>
       congr_app (extRen_tm xi_tm zeta_tm Eq_tm s0)
         (extRen_tm xi_tm zeta_tm Eq_tm s1)
@@ -121,7 +127,7 @@ Fixpoint compRenRen_tm (xi_tm : nat -> nat) (zeta_tm : nat -> nat)
 (rho_tm : nat -> nat) (Eq_tm : forall x, funcomp zeta_tm xi_tm x = rho_tm x)
 (s : tm) {struct s} : ren_tm zeta_tm (ren_tm xi_tm s) = ren_tm rho_tm s :=
   match s with
-  | var_tm s0 => ap var_tm (Eq_tm s0)
+  | var_tm s0 => ap (var_tm) (Eq_tm s0)
   | app s0 s1 =>
       congr_app (compRenRen_tm xi_tm zeta_tm rho_tm Eq_tm s0)
         (compRenRen_tm xi_tm zeta_tm rho_tm Eq_tm s1)
@@ -234,8 +240,8 @@ subst_tm tau_tm (subst_tm sigma_tm s) = subst_tm theta_tm s :=
   end.
 
 Lemma rinstInst_up_tm_tm (xi : nat -> nat) (sigma : nat -> tm)
-  (Eq : forall x, funcomp var_tm xi x = sigma x) :
-  forall x, funcomp var_tm (upRen_tm_tm xi) x = up_tm_tm sigma x.
+  (Eq : forall x, funcomp (var_tm) xi x = sigma x) :
+  forall x, funcomp (var_tm) (upRen_tm_tm xi) x = up_tm_tm sigma x.
 Proof.
 exact (fun n =>
        match n with
@@ -245,8 +251,8 @@ exact (fun n =>
 Qed.
 
 Fixpoint rinst_inst_tm (xi_tm : nat -> nat) (sigma_tm : nat -> tm)
-(Eq_tm : forall x, funcomp var_tm xi_tm x = sigma_tm x) (s : tm) {struct s} :
-ren_tm xi_tm s = subst_tm sigma_tm s :=
+(Eq_tm : forall x, funcomp (var_tm) xi_tm x = sigma_tm x) (s : tm) {struct s}
+   : ren_tm xi_tm s = subst_tm sigma_tm s :=
   match s with
   | var_tm s0 => Eq_tm s0
   | app s0 s1 =>
@@ -264,44 +270,64 @@ Proof.
 exact (compRenRen_tm xi_tm zeta_tm _ (fun n => eq_refl) s).
 Qed.
 
-Lemma compRen_tm (sigma_tm : nat -> tm) (zeta_tm : nat -> nat) (s : tm) :
+Lemma substRen_tm (sigma_tm : nat -> tm) (zeta_tm : nat -> nat) (s : tm) :
   ren_tm zeta_tm (subst_tm sigma_tm s) =
   subst_tm (funcomp (ren_tm zeta_tm) sigma_tm) s.
 Proof.
 exact (compSubstRen_tm sigma_tm zeta_tm _ (fun n => eq_refl) s).
 Qed.
 
-Lemma renComp_tm (xi_tm : nat -> nat) (tau_tm : nat -> tm) (s : tm) :
+Lemma renSubst_tm (xi_tm : nat -> nat) (tau_tm : nat -> tm) (s : tm) :
   subst_tm tau_tm (ren_tm xi_tm s) = subst_tm (funcomp tau_tm xi_tm) s.
 Proof.
 exact (compRenSubst_tm xi_tm tau_tm _ (fun n => eq_refl) s).
 Qed.
 
-Lemma compComp_tm (sigma_tm : nat -> tm) (tau_tm : nat -> tm) (s : tm) :
+Lemma substSubst_tm (sigma_tm : nat -> tm) (tau_tm : nat -> tm) (s : tm) :
   subst_tm tau_tm (subst_tm sigma_tm s) =
   subst_tm (funcomp (subst_tm tau_tm) sigma_tm) s.
 Proof.
 exact (compSubstSubst_tm sigma_tm tau_tm _ (fun n => eq_refl) s).
 Qed.
 
+Lemma rinstInst'_tm (xi_tm : nat -> nat) (s : tm) :
+  ren_tm xi_tm s = subst_tm (funcomp (var_tm) xi_tm) s.
+Proof.
+exact (rinst_inst_tm xi_tm _ (fun n => eq_refl) s).
+Qed.
+
+Lemma instId'_tm (s : tm) : subst_tm (var_tm) s = s.
+Proof.
+exact (idSubst_tm (var_tm) (fun n => eq_refl) s).
+Qed.
+
+Lemma rinstId'_tm (s : tm) : ren_tm id s = s.
+Proof.
+exact (eq_ind_r (fun t => t = s) (instId'_tm s) (rinstInst'_tm id s)).
+Qed.
+
+Lemma varL'_tm (sigma_tm : nat -> tm) (x : nat) :
+  subst_tm sigma_tm (var_tm x) = sigma_tm x.
+Proof.
+exact (eq_refl).
+Qed.
+
+Lemma varLRen'_tm (xi_tm : nat -> nat) (x : nat) :
+  ren_tm xi_tm (var_tm x) = var_tm (xi_tm x).
+Proof.
+exact (eq_refl).
+Qed.
+
 Class Up_tm X Y :=
     up_tm : X -> Y.
 
-Definition Subst_tm : Subst1 _ _ _ := @subst_tm.
+Instance Subst_tm : (Subst1 _ _ _) := @subst_tm.
 
-Existing Instance Subst_tm.
+Instance Up_tm_tm : (Up_tm _ _) := @up_tm_tm.
 
-Definition Up_tm_tm : Up_tm _ _ := @up_tm_tm.
+Instance Ren_tm : (Ren1 _ _ _) := @ren_tm.
 
-Existing Instance Up_tm_tm.
-
-Definition Ren_tm : Ren1 _ _ _ := @ren_tm.
-
-Existing Instance Ren_tm.
-
-Definition VarInstance_tm : Var _ _ := @var_tm.
-
-Existing Instance VarInstance_tm.
+Instance VarInstance_tm : (Var _ _) := @var_tm.
 
 Notation "[ sigma_tm ]" := (subst_tm sigma_tm)
   ( at level 1, left associativity, only printing) : fscope.
@@ -327,66 +353,21 @@ Notation "x '__tm'" := (@ids _ _ VarInstance_tm x)
 Notation "x '__tm'" := (var_tm x) ( at level 5, format "x __tm") :
   subst_scope.
 
-Lemma rinstInst_tm (xi_tm : nat -> nat) :
-  ren_tm xi_tm = subst_tm (funcomp var_tm xi_tm).
+Instance subst_tm_morphism :
+ (Proper (respectful (pointwise_relation _ eq) (respectful eq eq))
+    (@subst_tm)).
 Proof.
-exact (FunctionalExtensionality.functional_extensionality _ _
-         (fun x => rinst_inst_tm xi_tm _ (fun n => eq_refl) x)).
+exact (fun f_tm g_tm Eq_tm s t Eq_st =>
+       eq_ind s (fun t' => subst_tm f_tm s = subst_tm g_tm t')
+         (ext_tm f_tm g_tm Eq_tm s) t Eq_st).
 Qed.
 
-Lemma instId_tm : subst_tm var_tm = id.
+Instance ren_tm_morphism :
+ (Proper (respectful (pointwise_relation _ eq) (respectful eq eq)) (@ren_tm)).
 Proof.
-exact (FunctionalExtensionality.functional_extensionality _ _
-         (fun x => idSubst_tm var_tm (fun n => eq_refl) (id x))).
-Qed.
-
-Lemma rinstId_tm : @ren_tm id = id.
-Proof.
-exact (eq_trans (rinstInst_tm (id _)) instId_tm).
-Qed.
-
-Lemma varL_tm (sigma_tm : nat -> tm) :
-  funcomp (subst_tm sigma_tm) var_tm = sigma_tm.
-Proof.
-exact (FunctionalExtensionality.functional_extensionality _ _
-         (fun x => eq_refl)).
-Qed.
-
-Lemma varLRen_tm (xi_tm : nat -> nat) :
-  funcomp (ren_tm xi_tm) var_tm = funcomp var_tm xi_tm.
-Proof.
-exact (FunctionalExtensionality.functional_extensionality _ _
-         (fun x => eq_refl)).
-Qed.
-
-Lemma renRen'_tm (xi_tm : nat -> nat) (zeta_tm : nat -> nat) :
-  funcomp (ren_tm zeta_tm) (ren_tm xi_tm) = ren_tm (funcomp zeta_tm xi_tm).
-Proof.
-exact (FunctionalExtensionality.functional_extensionality _ _
-         (fun n => renRen_tm xi_tm zeta_tm n)).
-Qed.
-
-Lemma compRen'_tm (sigma_tm : nat -> tm) (zeta_tm : nat -> nat) :
-  funcomp (ren_tm zeta_tm) (subst_tm sigma_tm) =
-  subst_tm (funcomp (ren_tm zeta_tm) sigma_tm).
-Proof.
-exact (FunctionalExtensionality.functional_extensionality _ _
-         (fun n => compRen_tm sigma_tm zeta_tm n)).
-Qed.
-
-Lemma renComp'_tm (xi_tm : nat -> nat) (tau_tm : nat -> tm) :
-  funcomp (subst_tm tau_tm) (ren_tm xi_tm) = subst_tm (funcomp tau_tm xi_tm).
-Proof.
-exact (FunctionalExtensionality.functional_extensionality _ _
-         (fun n => renComp_tm xi_tm tau_tm n)).
-Qed.
-
-Lemma compComp'_tm (sigma_tm : nat -> tm) (tau_tm : nat -> tm) :
-  funcomp (subst_tm tau_tm) (subst_tm sigma_tm) =
-  subst_tm (funcomp (subst_tm tau_tm) sigma_tm).
-Proof.
-exact (FunctionalExtensionality.functional_extensionality _ _
-         (fun n => compComp_tm sigma_tm tau_tm n)).
+exact (fun f_tm g_tm Eq_tm s t Eq_st =>
+       eq_ind s (fun t' => ren_tm f_tm s = ren_tm g_tm t')
+         (extRen_tm f_tm g_tm Eq_tm s) t Eq_st).
 Qed.
 
 Ltac auto_unfold := repeat
@@ -400,57 +381,148 @@ Tactic Notation "auto_unfold" "in" "*" := repeat
                                             subst1 in *.
 
 Ltac asimpl' := repeat (first
-                 [ progress rewrite ?compComp'_tm
-                 | progress rewrite ?compComp_tm
-                 | progress rewrite ?renComp'_tm
-                 | progress rewrite ?renComp_tm
-                 | progress rewrite ?compRen'_tm
-                 | progress rewrite ?compRen_tm
-                 | progress rewrite ?renRen'_tm
+                 [ progress setoid_rewrite substSubst_tm
+                 | progress rewrite ?substSubst_tm
+                 | progress setoid_rewrite renSubst_tm
+                 | progress rewrite ?renSubst_tm
+                 | progress setoid_rewrite substRen_tm
+                 | progress rewrite ?substRen_tm
+                 | progress setoid_rewrite renRen_tm
                  | progress rewrite ?renRen_tm
-                 | progress rewrite ?varLRen_tm
-                 | progress rewrite ?varL_tm
-                 | progress rewrite ?rinstId_tm
-                 | progress rewrite ?instId_tm
+                 | progress setoid_rewrite varLRen'_tm
+                 | progress rewrite ?varLRen'_tm
+                 | progress setoid_rewrite varL'_tm
+                 | progress rewrite ?varL'_tm
+                 | progress setoid_rewrite rinstId'_tm
+                 | progress rewrite ?rinstId'_tm
+                 | progress setoid_rewrite instId'_tm
+                 | progress rewrite ?instId'_tm
                  | progress unfold up_tm_tm, upRen_tm_tm, up_ren
                  | progress cbn[subst_tm ren_tm]
-                 | fsimpl ]).
+                 | progress fsimpl
+                 | repeat unfold funcomp ]).
 
 Ltac asimpl := repeat try unfold_funcomp;
                 repeat
                  unfold VarInstance_tm, Var, ids, Ren_tm, Ren1, ren1,
                   Up_tm_tm, Up_tm, up_tm, Subst_tm, Subst1, subst1 in *;
-                asimpl'; repeat try unfold_funcomp.
+                asimpl'; minimize.
 
 Tactic Notation "asimpl" "in" hyp(J) := revert J; asimpl; intros J.
 
 Tactic Notation "auto_case" := auto_case ltac:(asimpl; cbn; eauto).
 
-Tactic Notation "asimpl" "in" "*" := repeat
-                                      unfold VarInstance_tm, Var, ids,
-                                       Ren_tm, Ren1, ren1, Up_tm_tm, Up_tm,
-                                       up_tm, Subst_tm, Subst1, subst1 
-                                       in *;
-                                      repeat (first
-                                       [ progress rewrite ?compComp'_tm in *
-                                       | progress rewrite ?compComp_tm in *
-                                       | progress rewrite ?renComp'_tm in *
-                                       | progress rewrite ?renComp_tm in *
-                                       | progress rewrite ?compRen'_tm in *
-                                       | progress rewrite ?compRen_tm in *
-                                       | progress rewrite ?renRen'_tm in *
-                                       | progress rewrite ?renRen_tm in *
-                                       | progress rewrite ?varLRen_tm in *
-                                       | progress rewrite ?varL_tm in *
-                                       | progress rewrite ?rinstId_tm in *
-                                       | progress rewrite ?instId_tm in *
-                                       | progress
-                                          unfold up_tm_tm, upRen_tm_tm,
-                                           up_ren in *
-                                       | progress cbn[subst_tm ren_tm] in *
-                                       | fsimpl ]).
+Ltac substify := auto_unfold; try repeat erewrite ?rinstInst'_tm.
 
-Ltac substify := auto_unfold; try repeat erewrite ?rinstInst_tm.
+Ltac renamify := auto_unfold; try repeat erewrite <- ?rinstInst'_tm.
 
-Ltac renamify := auto_unfold; try repeat erewrite <- ?rinstInst_tm.
+End renSubst.
+
+Module fext.
+
+Import
+renSubst.
+
+Lemma rinstInst_tm (xi_tm : nat -> nat) :
+  ren_tm xi_tm = subst_tm (funcomp (var_tm) xi_tm).
+Proof.
+exact (FunctionalExtensionality.functional_extensionality _ _
+         (fun x => rinst_inst_tm xi_tm _ (fun n => eq_refl) x)).
+Qed.
+
+Lemma instId_tm : subst_tm (var_tm) = id.
+Proof.
+exact (FunctionalExtensionality.functional_extensionality _ _
+         (fun x => idSubst_tm (var_tm) (fun n => eq_refl) (id x))).
+Qed.
+
+Lemma rinstId_tm : @ren_tm id = id.
+Proof.
+exact (eq_trans (rinstInst_tm (id _)) instId_tm).
+Qed.
+
+Lemma varL_tm (sigma_tm : nat -> tm) :
+  funcomp (subst_tm sigma_tm) (var_tm) = sigma_tm.
+Proof.
+exact (FunctionalExtensionality.functional_extensionality _ _
+         (fun x => eq_refl)).
+Qed.
+
+Lemma varLRen_tm (xi_tm : nat -> nat) :
+  funcomp (ren_tm xi_tm) (var_tm) = funcomp (var_tm) xi_tm.
+Proof.
+exact (FunctionalExtensionality.functional_extensionality _ _
+         (fun x => eq_refl)).
+Qed.
+
+Lemma renRen'_tm (xi_tm : nat -> nat) (zeta_tm : nat -> nat) :
+  funcomp (ren_tm zeta_tm) (ren_tm xi_tm) = ren_tm (funcomp zeta_tm xi_tm).
+Proof.
+exact (FunctionalExtensionality.functional_extensionality _ _
+         (fun n => renRen_tm xi_tm zeta_tm n)).
+Qed.
+
+Lemma substRen'_tm (sigma_tm : nat -> tm) (zeta_tm : nat -> nat) :
+  funcomp (ren_tm zeta_tm) (subst_tm sigma_tm) =
+  subst_tm (funcomp (ren_tm zeta_tm) sigma_tm).
+Proof.
+exact (FunctionalExtensionality.functional_extensionality _ _
+         (fun n => substRen_tm sigma_tm zeta_tm n)).
+Qed.
+
+Lemma renSubst'_tm (xi_tm : nat -> nat) (tau_tm : nat -> tm) :
+  funcomp (subst_tm tau_tm) (ren_tm xi_tm) = subst_tm (funcomp tau_tm xi_tm).
+Proof.
+exact (FunctionalExtensionality.functional_extensionality _ _
+         (fun n => renSubst_tm xi_tm tau_tm n)).
+Qed.
+
+Lemma substSubst'_tm (sigma_tm : nat -> tm) (tau_tm : nat -> tm) :
+  funcomp (subst_tm tau_tm) (subst_tm sigma_tm) =
+  subst_tm (funcomp (subst_tm tau_tm) sigma_tm).
+Proof.
+exact (FunctionalExtensionality.functional_extensionality _ _
+         (fun n => substSubst_tm sigma_tm tau_tm n)).
+Qed.
+
+Ltac asimpl_fext' := repeat (first
+                      [ progress setoid_rewrite substSubst_tm
+                      | progress setoid_rewrite renSubst_tm
+                      | progress setoid_rewrite substRen_tm
+                      | progress setoid_rewrite renRen_tm
+                      | progress setoid_rewrite substSubst'_tm
+                      | progress setoid_rewrite renSubst'_tm
+                      | progress setoid_rewrite substRen'_tm
+                      | progress setoid_rewrite renRen'_tm
+                      | progress setoid_rewrite varLRen_tm
+                      | progress setoid_rewrite varL_tm
+                      | progress setoid_rewrite rinstId_tm
+                      | progress setoid_rewrite instId_tm
+                      | progress unfold up_tm_tm, upRen_tm_tm, up_ren
+                      | progress cbn[subst_tm ren_tm]
+                      | fsimpl_fext ]).
+
+Ltac asimpl_fext := repeat try unfold_funcomp;
+                     repeat
+                      unfold VarInstance_tm, Var, ids, Ren_tm, Ren1, ren1,
+                       Up_tm_tm, Up_tm, up_tm, Subst_tm, Subst1, subst1 
+                       in *; asimpl_fext'; repeat try unfold_funcomp.
+
+Tactic Notation "asimpl_fext" "in" hyp(J) := revert J; asimpl_fext; intros J.
+
+Ltac substify_fext := auto_unfold; try repeat erewrite ?rinstInst_tm.
+
+Ltac renamify_fext := auto_unfold; try repeat erewrite <- ?rinstInst_tm.
+
+End fext.
+
+Module interface.
+
+Export renSubst.
+
+Export fext.
+
+End interface.
+
+Export interface.
 
