case-studies/kathrin/coq-setoid-funcomp/Chapter9/variadic_preservation.v
@@ -1,7 +1,7 @@
 (** ** Variadic Preservation *)
 
 Require Export ARS Program.Equality.
-Require Import core core_axioms fintype fintype_axioms.
+Require Import core fintype.
 Import ScopedNotations.
 From Chapter6 Require Export variadic_fin.
 Set Implicit Arguments.
@@ -24,11 +24,26 @@ Proof. intros ->. now constructor. Qed.
 
 (** *** Substitutivity *)
 
+(* TODO I also need this morphism to rewrite in a subsitution inside another substitution *)
+Require Import Setoid Morphisms.
+Instance subst_tm_morphism2  {m_tm : nat} {n_tm : nat}:
+ (Proper (pointwise_relation _ eq ==> pointwise_relation _ eq)
+    (@subst_tm m_tm n_tm)).
+Proof.
+  intros f g H s. now setoid_rewrite H.
+  Qed.
+
+Require Import core_axioms.
 Lemma step_inst {m n} (f : fin m -> tm n) (s t : tm m) :
   step s t -> step (subst_tm f s) (subst_tm f t).
 Proof.
   intros st. revert n f.  induction st; intros; cbn.
-  - apply step_beta'. now asimpl.
+  Hint Opaque scons_p : rewrite.
+  - apply step_beta'. asimpl.
+    unfold funcomp. setoid_rewrite scons_p_head'.
+    (* TODO a.d. why is cod_map not unfolded + why does the rewrite with scons_p_head' fail. It should happen in fsimpl *)
+    asimpl. unfold cod_map. asimpl.
+    reflexivity.
   - apply step_abs. eapply IHst.
   - apply step_appL, IHst.
 Qed.
